compcert_utils.v
@@ -45,6 +45,11 @@ Ltac rename_hyp1 h th :=
     | Mem.storev ?chk ?m ?vaddr ?v = ?m2 => fresh "heq_storev_" v
     | Mem.storev ?chk ?m ?vaddr ?v = ?m2 => fresh "heq_storev"
 
+    | Mem.unchanged_on ?prd ?m ?m' => fresh "h_unchanged_on_" prd "_" m "_" m'
+    | Mem.unchanged_on ?prd ?m ?m' => fresh "h_unchanged_on_" m "_" m'
+    | Mem.unchanged_on ?prd ?m ?m' => fresh "h_unchanged_on_" prd
+    | Mem.unchanged_on ?prd ?m ?m' => fresh "h_unchanged_on"
+
     | Globalenvs.Genv.find_funct ?g ?paddr = Some ?res => fresh "heq_find_func_" paddr "_" res
     | Globalenvs.Genv.find_funct ?g ?paddr = Some _ => fresh "heq_find_func_" paddr
     | Globalenvs.Genv.find_funct ?g _ = Some _ => fresh "heq_find_func"
